Notion of term context and contextual closure

pcuic/theories/PCUICReduction.v
@@ -1,10 +1,9 @@
 (* Distributed under the terms of the MIT license.   *)
 From Equations Require Import Equations.
-From Coq Require Import Bool String List Program BinPos Compare_dec Omega.
+From Coq Require Import Bool String List Program BinPos Compare_dec Omega Utf8.
 From Template Require Import config utils univ BasicAst.
 From PCUIC Require Import PCUICAst PCUICAstUtils PCUICInduction
-     PCUICLiftSubst PCUICUnivSubst PCUICTyping PCUICWeakeningEnv PCUICWeakening
-     PCUICSubstitution PCUICClosed.
+     PCUICLiftSubst PCUICUnivSubst PCUICTyping.
 Require Import ssreflect ssrbool.
 Require Import String.
 Require Import LibHypsNaming.
@@ -29,17 +28,175 @@ Proof.
   induction H; econstructor; eauto.
 Qed.
 
-(** Atoms do not reduce *)
+Lemma red_trans Σ Γ t u v : red Σ Γ t u -> red Σ Γ u v -> red Σ Γ t v.
+Proof.
+  intros. apply red_alt. apply red_alt in X. apply red_alt in X0. now econstructor 3.
+Defined.
+
+(** Atoms reduce to themselves *)
 
 Definition atom t :=
   match t with
+  | tRel _
   | tVar _
   | tMeta _
   | tSort _
+  | tConst _ _
   | tInd _ _
   | tConstruct _ _ _ => true
   | _ => false
   end.
+
+Section ReductionCongruence.
+  Context {Σ : global_context}.
+
+  (* Inductive list_context : list term -> list term -> term -> list term -> Type := *)
+  (* | list_context_head M MS : list_context (cons M MS) nil M MS *)
+  (* | list_context_cons MS Mleft M Mright M' : *)
+  (*     list_context MS Mleft M Mright -> *)
+  (*     list_context (cons M' MS) (cons M' Mleft) M Mright. *)
+  (* Derive NoConfusion for list_context. *)
+
+  (* TODO: fix lists *)
+
+  (* Inductive term_context : term -> Type := *)
+  (* | tHole M : term_context M *)
+  (* | tEvar_context n l lleft t lright : list_context l lleft t lright -> term_context (tEvar n l) *)
+  (* | tProd_context_dom na t t' : term_context t -> term_context (tProd na t t') *)
+  (* | tProd_context_codom na t t' : term_context t' -> term_context (tProd na t t') *)
+  (* | tLambda_context_dom na t t' : term_context t -> term_context (tLambda na t t') *)
+  (* | tLambda_context_codom na t t' : term_context t' -> term_context (tLambda na t t') *)
+  (* | tLetin_context_val na b t t' : term_context b -> term_context (tLetIn na b t t') *)
+  (* | tLetin_context_dom na b t t' : term_context t -> term_context (tLetIn na b t t') *)
+  (* | tLetin_context_codom na b t t' : term_context t' -> term_context (tLetIn na b t t') *)
+  (* | tApp_context_l f a : term_context f -> term_context (tApp f a) *)
+  (* | tApp_context_r f a : term_context a -> term_context (tApp f a) *)
+  (* (* missing Case/Proj/Fix/CoFix *). *)
+
+  Inductive term_context : Set :=
+  | tCtxHole : term_context
+  | tCtxEvar      : nat -> list_context -> term_context
+  | tCtxProd_l      : name -> term_context (* the type *) -> term -> term_context
+  | tCtxProd_r      : name -> term (* the type *) -> term_context -> term_context
+  | tCtxLambda_l    : name -> term_context (* the type *) -> term -> term_context
+  | tCtxLambda_r    : name -> term (* the type *) -> term_context -> term_context
+  | tCtxLetIn_l     : name -> term_context (* the term *) -> term (* the type *) ->
+                    term -> term_context
+  | tCtxLetIn_b     : name -> term (* the term *) -> term_context (* the type *) ->
+                    term -> term_context
+  | tCtxLetIn_r     : name -> term (* the term *) -> term (* the type *) ->
+                    term_context -> term_context
+  | tCtxApp_l       : term_context -> term -> term_context
+  | tCtxApp_r      : term -> term_context -> term_context
+  | tCtxCase_pred      : (inductive * nat) (* # of parameters *) -> term_context (* type info *)
+                         -> term (* discriminee *) -> list (nat * term) (* branches *) -> term_context
+  | tCtxCase_discr      : (inductive * nat) (* # of parameters *) -> term (* type info *)
+                 -> term_context (* discriminee *) -> list (nat * term) (* branches *) -> term_context
+  | tCtxCase_branch      : (inductive * nat) (* # of parameters *) -> term (* type info *)
+                           -> term (* discriminee *) -> list_nat_context (* branches *) -> term_context
+  | tCtxProj      : projection -> term_context -> term_context
+  | tCtxFix       : mfixpoint term -> nat -> term_context (* TODO *)
+  | tCtxCoFix     : mfixpoint term -> nat -> term_context (* TODO *)
+
+  with list_context : Set :=
+   | tCtxHead : term_context -> list term -> list_context
+   | tCtxTail : term -> list_context -> list_context
+
+  with list_nat_context : Set :=
+   | tCtxHead_nat : (nat * term_context) -> list (nat * term) -> list_nat_context
+   | tCtxTail_nat : (nat * term) -> list_nat_context -> list_nat_context.
+
+  Section FillContext.
+    Context (t : term).
+
+    Equations fill_context (ctx : term_context) (Γ : context) : term by struct ctx := {
+    | tCtxHole | Γ => t;
+    | tCtxEvar n l | Γ => tEvar n (fill_list_context l Γ);
+    | tCtxProd_l na ctx b | Γ => tProd na (fill_context ctx Γ) b;
+    | tCtxProd_r na ty ctx | Γ => tProd na ty (fill_context ctx (Γ ,, vass na ty));
+    | tCtxLambda_l na ty b | Γ => tLambda na (fill_context ty Γ) b;
+    | tCtxLambda_r na ty b | Γ => tLambda na ty (fill_context b (Γ ,, vass na ty));
+    | tCtxLetIn_l na b ty b' | Γ => tLetIn na (fill_context b Γ) ty b';
+    | tCtxLetIn_b na b ty b' | Γ => tLetIn na b (fill_context ty Γ) b';
+    | tCtxLetIn_r na b ty b' | Γ => tLetIn na b ty (fill_context b' (Γ ,, vdef na b ty));
+    | tCtxApp_l f a | Γ => tApp (fill_context f Γ) a;
+    | tCtxApp_r f a | Γ => tApp f (fill_context a Γ);
+    | tCtxCase_pred par p c brs | Γ => tCase par (fill_context p Γ) c brs;
+    | tCtxCase_discr par p c brs | Γ => tCase par p (fill_context c Γ) brs;
+    | tCtxCase_branch par p c brs | Γ => tCase par p c (fill_list_nat_context brs Γ);
+    | tCtxProj p c | Γ => tProj p (fill_context c Γ);
+    | tCtxFix mfix n | Γ => tFix mfix n;
+    | tCtxCoFix mfix n | Γ => tCoFix mfix n }
+    with fill_list_context (l : list_context) (Γ : context) : list term by struct l :=
+    { fill_list_context (tCtxHead ctx l) Γ => (fill_context ctx Γ) :: l;
+      fill_list_context (tCtxTail hd ctx) Γ => hd :: fill_list_context ctx Γ }
+    with fill_list_nat_context (l : list_nat_context) (Γ : context) : list (nat * term) by struct l :=
+    { fill_list_nat_context (tCtxHead_nat (n, ctx) l) Γ => (n, fill_context ctx Γ) :: l;
+      fill_list_nat_context (tCtxTail_nat hd ctx) Γ => hd :: fill_list_nat_context ctx Γ }.
+    Transparent fill_context fill_list_context fill_list_nat_context.
+  End FillContext.
+  Inductive contextual_closure (red : ∀ Γ, term -> term -> Type) : context -> term -> term -> Type :=
+  | ctxclos_atom Γ t : atom t -> contextual_closure red Γ t t
+  | ctxclos_ctx Γ (ctx : term_context) (c : context) (u u' : term) :
+      red (Γ ,,, c) u u' -> contextual_closure red Γ (fill_context u ctx c) (fill_context u' ctx c).
+
+  Lemma contextual_closure_red1 Γ t u : contextual_closure (red Σ) Γ t u -> red Σ Γ t u.
+  Proof.
+    induction 1. constructor.
+    revert u' r.
+    eapply (fill_context_elim (fun ctx u t => forall u', red Σ (Γ ,,, c) u u' ->
+                                                         red Σ Γ t (fill_context ctx u')) _ _);
+      intros **; simpl; auto.
+
+  Lemma red_abs {Γ : context} na M M' N N' : red Σ Γ M M' -> red Σ (Γ ,, vass na M) N N' ->
+                               red Σ Γ (tLambda na M N) (tLambda na M' N').
+  Proof.
+    intros.
+    induction X, X0; try constructor.
+    econstructor 2.
+
+
+
+
+  Lemma red_app M0 M1 N0 N1 :
+      red Σ Γ M0 M1 ->
+      red Σ Γ N0 N1 ->
+      red Σ Γ (tApp M0 N0) (tApp M1 N1)
+            (* do not handle mkApps yet *)
+  Lemma red_letin na d0 d1 t0 t1 b0 b1 :
+      red Σ Γ d0 d1 -> red Σ Γ t0 t1 -> red Σ (Γ ,, vdef na d0 t0) b0 b1 ->
+      red Σ Γ (tLetIn na d0 t0 b0) (tLetIn na d1 t1 b1)
+
+  Lemma red_case ind p0 p1 c0 c1 brs0 brs1 :
+      red Σ Γ p0 p1 ->
+      red Σ Γ c0 c1 ->
+      All2 (on_Trel (red Σ Γ) snd) brs0 brs1 ->
+      red Σ Γ (tCase ind p0 c0 brs0) (tCase ind p1 c1 brs1)
+
+  Lemma red_proj_congr p c c' : red Σ Γ c c' -> red Σ Γ (tProj p c) (tProj p c')
+
+  Lemma red_fix_congr mfix0 mfix1 idx :
+      All2 (fun d0 d1 => (red Σ Γ (dtype d0) (dtype d1)) *
+                         (red Σ (Γ ,,, fix_context mfix0) (dbody d0) (dbody d1)))%type mfix0 mfix1 ->
+      red Σ Γ (tFix mfix0 idx) (tFix mfix1 idx)
+
+  Lemma red_cofix_congr mfix0 mfix1 idx :
+      All2 (fun d0 d1 => (red Σ Γ (dtype d0) (dtype d1)) *
+                            (red Σ (Γ ,,, fix_context mfix0) (dbody d0) (dbody d1)))%type mfix0 mfix1 ->
+      red Σ Γ (tCoFix mfix0 idx) (tCoFix mfix1 idx)
+
+  Lemma red_prod na M0 M1 N0 N1 : red Σ Γ M0 M1 -> red Σ (Γ ,, vass na M0) N0 N1 ->
+                               red Σ Γ (tProd na M0 N0) (tProd na M1 N1)
+
+  Lemma red_evar Σ ev l l' : All2 (red Σ Γ) l l' -> red Σ Γ (tEvar ev l) (tEvar ev l')
+
+  Lemma red_atom t : atom t -> red Σ Γ t t.
+
+
+
+
+End ReductionCongruence.
+
 
 Section ParallelReduction.
   Context (Σ : global_declarations).
@@ -61,10 +218,6 @@ Section ParallelReduction.
       option_map decl_body (nth_error Γ i) = Some (Some body) ->
       pred1 Γ (lift0 (S i) body) body' ->
       pred1 Γ (tRel i) body'
-
-  | pred_rel_assum i :
-      option_map decl_body (nth_error Γ i) = Some None ->
-      pred1 Γ (tRel i) (tRel i)
 
   (** Case *)
   | pred_iota ind pars c u args0 args1 p brs0 brs1 :
@@ -104,10 +257,6 @@ Section ParallelReduction.
   | pred_delta c decl body (isdecl : declared_constant Σ c decl) u :
       decl.(cst_body) = Some body ->
       pred1 Γ (tConst c u) (subst_instance_constr u body)
-
-  | pred_axiom c decl (isdecl : declared_constant Σ c decl) u :
-      decl.(cst_body) = None ->
-      pred1 Γ (tConst c u) (tConst c u)
 
   (** Proj *)
   | pred_proj i pars narg args k u args0 args1 arg1 :
@@ -152,67 +301,201 @@ Section ParallelReduction.
 
   | pred_atom t : atom t -> pred1 Γ t t.
 
+  Definition All2_prop_relevant Γ {A} (f : A -> term) (rel1 : forall (t t' : term), pred1 Γ t t' -> Type) :=
+    All2 (fun x y => { red : pred1 Γ (f x) (f y) & rel1 (f x) (f y) red}).
+
+  Definition All2_prop Γ {A} (f : A -> term) (rel : forall (Γ : context) (t t' : term), Type) :=
+    All2 (on_Trel (rel Γ) f).
+
+  Definition All2_prop2 Γ Γ' {A} (f g : A -> term) (rel : forall (Γ : context) (t t' : term), Type) :=
+    All2 (fun x y => (on_Trel (rel Γ) f x y) * on_Trel (rel Γ') g x y)%type.
+
+  (* Scheme pred1_ind_all_first := Minimality for pred1 Sort Type. *)
+
+  Lemma All2_All2_prop {A} {P Q : context -> term -> term -> Type} {par} {f : A -> term} {l l' : list A} :
+    All2 (on_Trel (P par) f) l l' ->
+    (forall x y, P par x y -> Q par x y) ->
+    All2_prop par f Q l l'.
+  Proof.
+    intros H aux.
+    induction H; constructor. unfold on_Trel in *.
+    apply aux. apply r. apply IHAll2.
+  Defined.
+
+  Lemma All2_All2_prop2 {A} {P Q : context -> term -> term -> Type} {par par'} {f g : A -> term} {l l' : list A} :
+    All2_prop2 par par' f g P l l' ->
+    (forall par x y, P par x y -> Q par x y) ->
+    All2_prop2 par par' f g Q l l'.
+  Proof.
+    intros H aux.
+    induction H; constructor. unfold on_Trel in *. split.
+    apply aux. destruct r. apply p. apply aux. apply r. apply IHAll2.
+  Defined.
+
+  Definition extendP {P Q: context -> term -> term -> Type} (aux : forall Γ t t', P Γ t t' -> Q Γ t t') :
+    (forall Γ t t', P Γ t t' -> (P Γ t t' * Q Γ t t')).
+  Proof.
+    intros. split. apply X. apply aux. apply X.
+  Defined.
+
+  Lemma pred1_ind_all :
+    forall P : forall (Γ : context) (t t0 : term), Type,
+      let P' Γ x y := ((pred1 Γ x y) * P Γ x y)%type in
+      (forall (Γ : context) (na : name) (t b0 b1 a0 a1 : term),
+          pred1 Γ b0 b1 -> P Γ b0 b1 -> pred1 Γ a0 a1 -> P Γ a0 a1 -> P Γ (tApp (tLambda na t b0) a0) (b1 {0 := a1})) ->
+      (forall (Γ : context) (na : name) (d0 d1 t b0 b1 : term),
+          pred1 Γ d0 d1 -> P Γ d0 d1 -> pred1 Γ b0 b1 -> P Γ b0 b1 -> P Γ (tLetIn na d0 t b0) (b1 {0 := d1})) ->
+      (forall (Γ : context) (i : nat) (body body' : term),
+          option_map decl_body (nth_error Γ i) = Some (Some body) ->
+          pred1 Γ ((lift0 (S i)) body) body' -> P Γ ((lift0 (S i)) body) body' -> P Γ (tRel i) body') ->
+      (forall (Γ : context) (ind : inductive) (pars c : nat) (u : universe_instance) (args0 args1 : list term)
+              (p : term) (brs0 brs1 : list (nat * term)),
+          All2_prop Γ id P' args0 args1 ->
+          All2_prop Γ snd P' brs0 brs1 ->
+          P Γ (tCase (ind, pars) p (mkApps (tConstruct ind c u) args0) brs0) (iota_red pars c args1 brs1)) ->
+      (forall (Γ : context) (mfix : mfixpoint term) (idx : nat) (args0 args1 : list term) (narg : nat) (fn0 fn1 : term),
+          unfold_fix mfix idx = Some (narg, fn0) ->
+          is_constructor narg args1 = true ->
+          All2_prop Γ id P' args0 args1 ->
+          pred1 Γ fn0 fn1 -> P Γ fn0 fn1 -> P Γ (mkApps (tFix mfix idx) args0) (mkApps fn1 args1)) ->
+      (forall (Γ : context) (ip : inductive * nat) (p0 p1 : term) (mfix : mfixpoint term) (idx : nat)
+              (args0 args1 : list term) (narg : nat) (fn0 fn1 : term) (brs0 brs1 : list (nat * term)),
+          unfold_cofix mfix idx = Some (narg, fn0) ->
+          All2_prop Γ id P' args0 args1 ->
+          pred1 Γ fn0 fn1 ->
+          P Γ fn0 fn1 ->
+          pred1 Γ p0 p1 ->
+          P Γ p0 p1 ->
+          All2_prop Γ snd P' brs0 brs1 ->
+          P Γ (tCase ip p0 (mkApps (tCoFix mfix idx) args0) brs0) (tCase ip (mkApps fn1 args1) p1 brs1)) ->
+      (forall (Γ : context) (p : projection) (mfix : mfixpoint term) (idx : nat) (args0 args1 : list term)
+              (narg : nat) (fn0 fn1 : term),
+          unfold_cofix mfix idx = Some (narg, fn0) ->
+          All2_prop Γ id P' args0 args1 ->
+          pred1 Γ fn0 fn1 -> P Γ fn0 fn1 -> P Γ (tProj p (mkApps (tCoFix mfix idx) args0)) (tProj p (mkApps fn1 args1))) ->
+      (forall (Γ : context) (c : ident) (decl : constant_body) (body : term),
+          declared_constant Σ c decl ->
+          forall u : universe_instance, cst_body decl = Some body -> P Γ (tConst c u) (subst_instance_constr u body)) ->
+      (forall (Γ : context) (i : inductive) (pars narg : nat) (args : list term) (k : nat) (u : universe_instance)
+              (args0 args1 : list term) (arg1 : term),
+          All2_prop Γ id P' args0 args1 ->
+          nth_error args (pars + narg) = Some arg1 -> P Γ (tProj (i, pars, narg) (mkApps (tConstruct i k u) args0)) arg1) ->
+      (forall (Γ : context) (na : name) (M M' N N' : term),
+          pred1 Γ M M' ->
+          P Γ M M' -> pred1 (Γ,, vass na M) N N' -> P (Γ,, vass na M) N N' -> P Γ (tLambda na M N) (tLambda na M' N')) ->
+      (forall (Γ : context) (M0 M1 N0 N1 : term),
+          pred1 Γ M0 M1 -> P Γ M0 M1 -> pred1 Γ N0 N1 -> P Γ N0 N1 -> P Γ (tApp M0 N0) (tApp M1 N1)) ->
+      (forall (Γ : context) (na : name) (d0 d1 t0 t1 b0 b1 : term),
+          pred1 Γ d0 d1 ->
+          P Γ d0 d1 ->
+          pred1 Γ t0 t1 ->
+          P Γ t0 t1 ->
+          pred1 (Γ,, vdef na d0 t0) b0 b1 -> P (Γ,, vdef na d0 t0) b0 b1 -> P Γ (tLetIn na d0 t0 b0) (tLetIn na d1 t1 b1)) ->
+      (forall (Γ : context) (ind : inductive * nat) (p0 p1 c0 c1 : term) (brs0 brs1 : list (nat * term)),
+          pred1 Γ p0 p1 ->
+          P Γ p0 p1 ->
+          pred1 Γ c0 c1 ->
+          P Γ c0 c1 -> All2_prop Γ snd P' brs0 brs1 -> P Γ (tCase ind p0 c0 brs0) (tCase ind p1 c1 brs1)) ->
+      (forall (Γ : context) (p : projection) (c c' : term), pred1 Γ c c' -> P Γ c c' -> P Γ (tProj p c) (tProj p c')) ->
+      (forall (Γ : context) (mfix0 : mfixpoint term) (mfix1 : list (def term)) (idx : nat),
+          All2_prop2 Γ (Γ ,,, fix_context mfix0) dtype dbody P' mfix0 mfix1 ->
+          P Γ (tFix mfix0 idx) (tFix mfix1 idx)) ->
+      (forall (Γ : context) (mfix0 : mfixpoint term) (mfix1 : list (def term)) (idx : nat),
+          All2_prop2 Γ (Γ ,,, fix_context mfix0) dtype dbody P' mfix0 mfix1 ->
+          P Γ (tCoFix mfix0 idx) (tCoFix mfix1 idx)) ->
+      (forall (Γ : context) (na : name) (M0 M1 N0 N1 : term),
+          pred1 Γ M0 M1 ->
+          P Γ M0 M1 -> pred1 (Γ,, vass na M0) N0 N1 -> P (Γ,, vass na M0) N0 N1 -> P Γ (tProd na M0 N0) (tProd na M1 N1)) ->
+      (forall (Γ : context) (ev : nat) (l l' : list term), All2_prop Γ id P' l l' -> P Γ (tEvar ev l) (tEvar ev l')) ->
+      (forall (Γ : context) (t : term), atom t -> P Γ t t) ->
+      forall (Γ : context) (t t0 : term), pred1 Γ t t0 -> P Γ t t0.
+  Proof.
+    intros. revert Γ t t0 X18.
+    fix aux 4. intros Γ t t'.
+    move aux at top.
+    destruct 1; match goal with
+                | |- P _ (tFix _ _) (tFix _ _) => idtac
+                | |- P _ (tCoFix _ _) (tCoFix _ _) => idtac
+                | |- P _ (mkApps (tFix _ _) _) _ => idtac
+                | |- P _ (tCase _ _ (mkApps (tCoFix _ _) _) _) _ => idtac
+                | |- P _ (tProj _ (mkApps (tCoFix _ _) _)) _ => idtac
+                | H : _ |- _ => eapply H; eauto
+                end.
+    - apply (All2_All2_prop (P:=pred1) (Q:=P') (f:=id) a ((extendP aux) Γ)).
+    - apply (All2_All2_prop (P:=pred1) (Q:=P') (f:=snd) a0 (extendP aux Γ)).
+    - eapply X3; eauto.
+      eapply (All2_All2_prop (P:=pred1) (Q:=P') (f:=id) a (extendP aux Γ)).
+    - eapply X4; eauto.
+      eapply (All2_All2_prop (P:=pred1) (Q:=P') (f:=id) a (extendP aux Γ)).
+      eapply (All2_All2_prop (P:=pred1) (Q:=P') (f:=snd) a0 (extendP aux Γ)).
+    - eapply X5; eauto.
+      eapply (All2_All2_prop (P:=pred1) (Q:=P') (f:=id) a (extendP aux Γ)).
+    - eapply (All2_All2_prop (P:=pred1) (Q:=P') (f:=id) a (extendP aux Γ)).
+    - eapply (All2_All2_prop (P:=pred1) (Q:=P') (f:=snd) a (extendP aux Γ)).
+    - eapply X13.
+      eapply (All2_All2_prop2 (P:=pred1) (Q:=P') (f:=dtype) (g:=dbody) a (extendP aux)).
+    - eapply X14.
+      eapply (All2_All2_prop2 (P:=pred1) (Q:=P') (f:=dtype) (g:=dbody) a (extendP aux)).
+    - eapply (All2_All2_prop (P:=pred1) (Q:=P') (f:=id) a (extendP aux Γ)).
+  Defined.
+
+  Hint Resolve All_All2 : all.
+
   Lemma pred1_refl Γ t : pred1 Γ t t.
   Proof.
     induction t in Γ |- * using term_forall_list_ind;
-      try solve [(apply pred_atom; reflexivity) || constructor; auto].
-    constructor. solve_all; eapply All_Forall2; eauto. simpl. auto.
-    econstructor; auto. solve_all. eapply All_Forall2; eauto. simpl; auto.
-    constructor; eauto. red in H. solve_all. eapply All_Forall2; eauto. simpl; intuition auto.
-    red. auto.
-    constructor; eauto. red in H. solve_all. eapply All_Forall2; eauto. simpl; intuition auto.
-    constructor; eauto. red in H. solve_all. eapply All_Forall2; eauto. simpl; intuition auto.
+      try solve [(apply pred_atom; reflexivity) || constructor; auto];
+      try solve [constructor; unfold on_Trel; solve_all].
   Qed.
 
   Hint Constructors pred1 : pred.
   Hint Resolve pred1_refl : pred.
 
-  Lemma Forall2_same {A} (P : A -> A -> Prop) l : (forall x, P x x) -> Forall2 P l l.
+  Lemma All2_same {A} (P : A -> A -> Type) l : (forall x, P x x) -> All2 P l l.
   Proof. induction l; constructor; auto. Qed.
 
-  Hint Resolve Forall2_same : pred.
-  Hint Unfold on_rel snd on_snd : pred.
+  Hint Resolve All2_same : pred.
+  Hint Unfold on_rel on_Trel snd on_snd : pred.
+
+  Lemma OnOne2_All2 {A}:
+    forall (ts ts' : list A) P Q,
+      OnOne2 P ts ts' ->
+      (forall x y, P x y -> Q x y)%type ->
+      (forall x, Q x x) ->
+      All2 Q ts ts'.
+  Proof.
+    intros ts ts' P Q X.
+    induction X; intuition auto with pred.
+  Qed.
+
+  Ltac OnOne2_All2 :=
+    match goal with
+      | [ H : OnOne2 ?P ?ts ?ts' |- All2 ?Q ?ts ?ts' ] =>
+        unshelve eapply (OnOne2_All2 _ _ P Q H); simpl; intros
+    end.
+
+  Hint Extern 0 (All2 _ _ _) => OnOne2_All2; intuition auto with pred : pred.
 
   Lemma red1_pred1 Γ : forall M N, red1 Σ Γ M N -> pred1 Γ M N.
-    induction 1 using red1_ind_all; intros; eauto with pred.
+    induction 1 using red1_ind_all; intros; eauto with pred;
+      try solve [constructor; intuition auto with pred].
 
-    constructor; auto with pred.
-    induction H. intuition. constructor; auto with pred.
-    admit.
+    constructor; auto with pred. OnOne2_All2; intuition auto with pred. rewrite b0. auto with pred.
+    constructor; auto with pred. OnOne2_All2; intuition auto with pred. rewrite b0. auto with pred.
+    constructor; auto with pred. OnOne2_All2; intuition auto with pred. rewrite b0. auto with pred.
+    constructor; auto with pred. OnOne2_All2; intuition auto with pred. rewrite b0. auto with pred.
+  Qed.
 
-    constructor. auto with pred.
-    induction H. constructor; intuition auto with pred.
-    constructor; auto with pred.
-    constructor; auto with pred.
-
-    induction H; constructor; intuition auto with pred.
-
-    constructor.
-    generalize (fix_context mfix0).
-    induction H; constructor; intuition auto with pred.
-    rewrite H1; auto with pred.
-
-    constructor.
-    revert H.
-    generalize (fix_context mfix0).
-    induction 1; constructor; intuition auto with pred.
-    rewrite H1; auto with pred.
-
-    constructor.
-    generalize (fix_context mfix0).
-    induction H; constructor; intuition auto with pred.
-    rewrite H1; auto with pred.
-
-    constructor.
-    revert H.
-    generalize (fix_context mfix0).
-    induction 1; constructor; intuition auto with pred.
-    rewrite H1; auto with pred.
-  Admitted.
-
+  (** Parallel reduction is included in the reflexive transitive closure of 1-step reduction *)
   Lemma pred1_red Γ : forall M N, pred1 Γ M N -> red Σ Γ M N.
   Proof.
-    induction 1; try constructor; auto with pred.
+    revert Γ. eapply pred1_ind_all; intros; try constructor; auto with pred.
+
+    - apply red_trans with (tApp (tLambda na t b1) a0).
+      apply
+
+
+
   Admitted.
 
 End ParallelReduction.
